HOL/SepLogic/Dijkstra_Impl.thy
@@ -1,5 +1,5 @@
 theory Dijkstra_Impl
-imports IndexedPriorityQueue "../DataStrs/Dijkstra"
+imports Indexed_PQueue_Impl "../DataStrs/Dijkstra"
 begin
 
 datatype dijkstra_state = Dijkstra_State (est_a: "nat array") (heap_pq: "nat indexed_pqueue")
